reboot composition in CPS with explicit context coverings

theories/STLC/Ctx.v
@@ -2,6 +2,7 @@ Import EqNotations.
 From ExtLib.Data Require Import Nat Fin List.
 From Equations Require Import Equations.
 From OGS Require Import Utils.
+Set Equations Transparent.
 
 Definition ctx (X : Type) : Type := list X.
 
@@ -87,5 +88,108 @@ Equations r_concat3_2 (Γ Δ ϒ : ctx X) : forall t, (Γ +▶ ϒ) ∋ t -> (Γ +
   r_concat3_2 Γ Δ (ϒ ▶ _) _ (pop i) := pop (r_concat3_2 Γ Δ ϒ _ i) .
 Arguments r_concat3_2 {Γ Δ ϒ}.
 
+Variant any (P : X -> Type) (xs : list X) : Type :=
+| Any {x} : xs ∋ x -> P x -> any P xs
+.
+Arguments Any {P xs x} i p.
+
+Equations any_el {P xs} : any P xs -> X :=
+  any_el (@Any _ _ x _ _) := x .
+
+Equations any_coh {P xs} (a : any P xs) : P (any_el a) :=
+  any_coh (Any _ p) := p .
+
+Equations any_elim {P} {A : forall x, P x -> Type} (f : forall x p, A x p)
+          xs (a : any P xs) : A (any_el a) (any_coh a) :=
+  any_elim f xs (Any _ p) := f _ p .
+
+Inductive cover : ctx X -> ctx X -> ctx X -> Type :=
+| CNil :                                 cover ∅        ∅        ∅
+| CLeft {x xs ys zs} : cover xs ys zs ->  cover (xs ▶ x) ys       (zs ▶ x)
+| CRight {x xs ys zs} : cover xs ys zs -> cover xs       (ys ▶ x) (zs ▶ x)
+.
+Arguments CNil.
+Arguments CLeft {x xs ys zs} c.
+Arguments CRight {x xs ys zs} c.
+Notation "a ⊎ b ≡ c" := (cover a b c) (at level 30).
+
+Equations cover_nil_r xs : xs ⊎ ∅ ≡ xs :=
+  cover_nil_r ∅        := CNil ;
+  cover_nil_r (xs ▶ x) := CLeft (cover_nil_r xs) .
+#[global] Arguments cover_nil_r {xs}.
+
+Equations cover_nil_l xs : ∅ ⊎ xs ≡ xs :=
+  cover_nil_l ∅        := CNil ;
+  cover_nil_l (xs ▶ x) := CRight (cover_nil_l xs) .
+#[global] Arguments cover_nil_l {xs}.
+
+Equations cover_cat {xs} ys : xs ⊎ ys ≡ (xs +▶ ys) :=
+  cover_cat ∅        := cover_nil_r ;
+  cover_cat (ys ▶ y) := CRight (cover_cat ys) .
+#[global] Arguments cover_cat {xs ys}.
+
+Equations cat_cover {xs0 xs1 ys0 ys1 zs0 zs1} : xs0 ⊎ ys0 ≡ zs0 -> xs1 ⊎ ys1 ≡ zs1
+    -> (xs0 +▶ xs1) ⊎ (ys0 +▶ ys1) ≡ (zs0 +▶ zs1) :=
+  cat_cover a (CNil)     := a ;
+  cat_cover a (CLeft b)  := CLeft (cat_cover a b) ;
+  cat_cover a (CRight b) := CRight (cat_cover a b) .
+
+Equations ext_cover_l {xs ys zs} (u : ctx X) : xs ⊎ ys ≡ zs -> (xs +▶ u) ⊎ ys ≡ (zs +▶ u) :=
+  ext_cover_l ∅ c := c ; 
+  ext_cover_l (uu ▶ _) c := CLeft (ext_cover_l uu c) .
+
+Equations ext_cover_r {xs ys zs} (u : ctx X) : xs ⊎ ys ≡ zs -> xs ⊎ (ys +▶ u) ≡ (zs +▶ u) :=
+  ext_cover_r ∅ c := c ; 
+  ext_cover_r (uu ▶ _) c := CRight (ext_cover_r uu c) .
+
+Equations r_cover_l {xs ys zs} (p : xs ⊎ ys ≡ zs) [x] : xs ∋ x -> zs ∋ x :=
+  r_cover_l (CLeft c)  top     := top ;
+  r_cover_l (CLeft c)  (pop i) := pop (r_cover_l c i) ;
+  r_cover_l (CRight c) i       := pop (r_cover_l c i) .
+
+Equations r_cover_r {xs ys zs} (p : xs ⊎ ys ≡ zs) [x] : ys ∋ x -> zs ∋ x :=
+  r_cover_r (CLeft c)  i       := pop (r_cover_r c i) ;
+  r_cover_r (CRight c) top     := top ;
+  r_cover_r (CRight c) (pop i) := pop (r_cover_r c i) .
+
+Equations cover_split {xs ys zs} (p : xs ⊎ ys ≡ zs) [x] : zs ∋ x -> xs ∋ x + ys ∋ x:=
+  cover_split (CLeft c)  top     := inl top ;
+  cover_split (CRight c) top     := inr top ;
+  cover_split (CLeft c)  (pop i) with cover_split c i :=
+      { | inl j := inl (pop j) ;
+        | inr j := inr j } ;
+  cover_split (CRight c) (pop i) with cover_split c i :=
+      { | inl j := inl j ;
+        | inr j := inr (pop j) } .
+
+Equations any_c_split {P xs ys zs} : xs ⊎ ys ≡ zs -> any P zs -> any P xs + any P ys :=
+  any_c_split c (Any i p) with cover_split c i :=
+    { | inl j := inl (Any j p) ;
+      | inr j := inr (Any j p) } .
+
+Equations r_any {P xs ys} (ρ : forall x, xs ∋ x -> ys ∋ x) : any P xs -> any P ys :=
+  r_any ρ (Any i p) := Any (ρ _ i) p .
+
+(*
+Equations any_c_split_coh1 {P xs ys zs} (c : xs ⊎ ys ≡ zs) (a : any P zs) :
+  any_el a = match any_c_split c a with
+             | inl a' => any_el a'
+             | inr a' => any_el a'
+             end :=
+  any_c_split_coh1 c (@Any _ _ x i p) with cover_split c i :=
+    { | inl j := eq_refl ;
+      | inr j := eq_refl } .
+
+Equations any_c_split_coh2 {P xs ys zs} (c : xs ⊎ ys ≡ zs) (a : any P zs) :
+  any_el a = match any_c_split c a with
+             | inl a' => any_el a'
+             | inr a' => any_el a'
+             end :=
+  any_c_split_coh1 c (@Any _ _ x i p) with cover_split c i :=
+    { | inl j := eq_refl ;
+      | inr j := eq_refl } .
+*)
+
 End lemma.
 #[global] Notation "Γ ∋ x" := (has Γ%ctx x) (at level 30).
+#[global] Notation "a ⊎ b ≡ c" := (cover a b c) (at level 30).
